riscV/Asmgenproof.v
@@ -1516,16 +1516,16 @@ Local Transparent destroyed_by_op.
     unfold Genv.find_comp; simpl; rewrite FIND;
       destruct Ptrofs.eq_dec; try congruence. }
   econstructor. traceEq. traceEq.
-  destruct (Genv.type_of_call ge (Mach.call_comp ge s) (comp_of f)) eqn:TY_CALL.
-  {
-  replace (Mach.fn_sig f) with (fn_sig tf).
-  econstructor; eauto.
-  rewrite X; simpl; Simpl; eauto.
+  (* destruct (Genv.type_of_call ge (Mach.call_comp ge s) (comp_of f)) eqn:TY_CALL. *)
+  (* { *)
+  (* replace (Mach.fn_sig f) with (fn_sig tf). *)
+  (* econstructor; eauto. *)
+  (* rewrite X; simpl; Simpl; eauto. *)
 
-  apply agree_set_other; auto with asmgen.
-  { monadInv H5. destruct (zlt Ptrofs.max_unsigned (list_length_z (fn_code x0))); try discriminate.
-    inv EQ1. monadInv EQ0. reflexivity. }
-  }
+  (* apply agree_set_other; auto with asmgen. *)
+  (* { monadInv H5. destruct (zlt Ptrofs.max_unsigned (list_length_z (fn_code x0))); try discriminate. *)
+  (*   inv EQ1. monadInv EQ0. reflexivity. } *)
+  (* } *)
   { (* new case *)
 
   replace (Mach.fn_sig f) with (fn_sig tf).
@@ -1542,15 +1542,15 @@ Local Transparent destroyed_by_op.
   { monadInv H5. destruct (zlt Ptrofs.max_unsigned (list_length_z (fn_code x0))); try discriminate.
     inv EQ1. monadInv EQ0. reflexivity. }
   }
-  { (* same as Genv.InternalCall *)
-  replace (Mach.fn_sig f) with (fn_sig tf).
-  econstructor; eauto.
-  rewrite X; simpl; Simpl; eauto.
+  (* { (* same as Genv.InternalCall *) *)
+  (* replace (Mach.fn_sig f) with (fn_sig tf). *)
+  (* econstructor; eauto. *)
+  (* rewrite X; simpl; Simpl; eauto. *)
 
-  apply agree_set_other; auto with asmgen.
-  { monadInv H5. destruct (zlt Ptrofs.max_unsigned (list_length_z (fn_code x0))); try discriminate.
-    inv EQ1. monadInv EQ0. reflexivity. }
-  }
+  (* apply agree_set_other; auto with asmgen. *)
+  (* { monadInv H5. destruct (zlt Ptrofs.max_unsigned (list_length_z (fn_code x0))); try discriminate. *)
+  (*   inv EQ1. monadInv EQ0. reflexivity. } *)
+  (* } *)
 
 - (* internal function *)
   (* assert (cp = comp_of f). *)
@@ -1599,22 +1599,22 @@ Local Transparent destroyed_by_op.
   left; eexists; split.
   eapply exec_straight_steps_1; eauto. lia. simpl. unfold Genv.find_comp; simpl.
   now rewrite A. constructor.
-  destruct (Genv.type_of_call ge (Mach.call_comp ge s) (Genv.find_comp ge (Vptr fb Ptrofs.zero))) eqn:TY_CALL.
-  {
-  econstructor; eauto.
-  { rewrite X, <- STACKS_COMP, ATPC. reflexivity. }
-  (* rewrite X. rewrite ATPC in STACKS'. eapply match_stacks_same_compartment; eauto. *)
-  rewrite X; econstructor; eauto.
-  apply agree_exten with rs2; eauto with asmgen.
-  unfold rs2.
-  apply agree_nextinstr. apply agree_set_other; auto with asmgen.
-  apply agree_change_sp with (parent_sp s).
-  apply agree_undef_regs with rs0. auto.
-Local Transparent destroyed_at_function_entry.
-  simpl; intros; Simpl.
-  unfold sp; congruence.
-  intros. rewrite V by auto with asmgen. reflexivity.
-  }
+(*   destruct (Genv.type_of_call ge (Mach.call_comp ge s) (Genv.find_comp ge (Vptr fb Ptrofs.zero))) eqn:TY_CALL. *)
+(*   { *)
+(*   econstructor; eauto. *)
+(*   { rewrite X, <- STACKS_COMP, ATPC. reflexivity. } *)
+(*   (* rewrite X. rewrite ATPC in STACKS'. eapply match_stacks_same_compartment; eauto. *) *)
+(*   rewrite X; econstructor; eauto. *)
+(*   apply agree_exten with rs2; eauto with asmgen. *)
+(*   unfold rs2. *)
+(*   apply agree_nextinstr. apply agree_set_other; auto with asmgen. *)
+(*   apply agree_change_sp with (parent_sp s). *)
+(*   apply agree_undef_regs with rs0. auto. *)
+(* Local Transparent destroyed_at_function_entry. *)
+(*   simpl; intros; Simpl. *)
+(*   unfold sp; congruence. *)
+(*   intros. rewrite V by auto with asmgen. reflexivity. *)
+(*   } *)
   { (* new case*)
   econstructor; eauto.
   { rewrite X, <- STACKS_COMP, ATPC. reflexivity. }
@@ -1635,21 +1635,21 @@ Local Transparent destroyed_at_function_entry.
   unfold sp; congruence.
   intros. rewrite V by auto with asmgen. reflexivity.
   }
-  { (* same as Genv.InternalCall *)
-  econstructor; eauto.
-  { rewrite X, <- STACKS_COMP, ATPC. reflexivity. }
-  (* rewrite X. rewrite ATPC in STACKS'. eapply match_stacks_same_compartment; eauto. *)
-  rewrite X; econstructor; eauto.
-  apply agree_exten with rs2; eauto with asmgen.
-  unfold rs2.
-  apply agree_nextinstr. apply agree_set_other; auto with asmgen.
-  apply agree_change_sp with (parent_sp s).
-  apply agree_undef_regs with rs0. auto.
-Local Transparent destroyed_at_function_entry.
-  simpl; intros; Simpl.
-  unfold sp; congruence.
-  intros. rewrite V by auto with asmgen. reflexivity.
-  }
+(*   { (* same as Genv.InternalCall *) *)
+(*   econstructor; eauto. *)
+(*   { rewrite X, <- STACKS_COMP, ATPC. reflexivity. } *)
+(*   (* rewrite X. rewrite ATPC in STACKS'. eapply match_stacks_same_compartment; eauto. *) *)
+(*   rewrite X; econstructor; eauto. *)
+(*   apply agree_exten with rs2; eauto with asmgen. *)
+(*   unfold rs2. *)
+(*   apply agree_nextinstr. apply agree_set_other; auto with asmgen. *)
+(*   apply agree_change_sp with (parent_sp s). *)
+(*   apply agree_undef_regs with rs0. auto. *)
+(* Local Transparent destroyed_at_function_entry. *)
+(*   simpl; intros; Simpl. *)
+(*   unfold sp; congruence. *)
+(*   intros. rewrite V by auto with asmgen. reflexivity. *)
+(*   } *)
 
 - (* external function *)
   exploit functions_translated; eauto.
